src/tls/TLS.Handshake.fst
@@ -27,6 +27,12 @@ module KS = Old.KeySchedule
 module HMAC_UFCMA = Old.HMAC.UFCMA
 module HSM = HandshakeMessages
 
+module Client = TLS.Handshake.Client
+module Server = TLS.Handshake.Server
+module PF = TLS.Handshake.ParseFlights
+
+module LP = LowParse.Low.Base
+
 // consider adding an optional (resume: option sid) on the client side
 // for now this bit is not explicitly authenticated.
 
@@ -40,35 +46,46 @@ module HSM = HandshakeMessages
 // abstract invariant; depending only on the HS state (not the epochs state)
 // no need for an epoch states invariant here: the HS never modifies them
 
-#set-options "--admit_smt_queries true"
-
-let is_0rtt hs = admit()
+let is_0rtt_offered hs = admit()
 
 let xkeys_of hs = 
   let n = Machine.nonce hs in 
   FStar.Monotonic.Seq.i_read (Machine.epochs hs n).Epochs.exporter
 
+open TLS.Handshake.Machine 
+
+
+/// now integrating Outline.fst; see also
+/// https://github.com/project-everest/mitls-fstar/issues/231 and
+/// https://github.com/project-everest/mitls-fstar/blob/afromher_dev/src/tls/Test.TLS.Send.fst
+
 (* -------------------- Control Interface ---------------------- *)
 
+//19-09-11 we'll need to split it between clients and servers, since their config differ. 
+
 let create (parent:rid) cfg role =
+  assert(role == TLSConstants.Client);
   let r = new_region parent in
-  let log = HSL.create r None (* cfg.max_version (Nego.hashAlg nego) *) in
+  // let log = HSL.create r None (* cfg.max_version (Nego.hashAlg nego) *) in
   //let nonce = Nonce.mkHelloRandom r r0 in //NS: should this really be Client?
   let ks, nonce = KS.create #r role cfg.is_quic in
-  let nego = Nego.create r role cfg nonce in
-  let epochs = Epochs.create r nonce in
-  let state = ralloc r (if role = Client then C_init else S_Idle) in
-  let x: hs = HS role nego log ks epochs state in //17-04-17 why needed?
-  x
+  // let nego = Nego.create r role cfg nonce in
+  // let epochs = Epochs.create r nonce in
+  let resume = None, [] in //TODO 19-09-13 cfg.use_tickets in 
+  let config: client_config = cfg, resume in 
+  let state = ralloc r (C_init nonce) in
+  Machine.Client r config state
 
 let rehandshake s c = FStar.Error.unexpected "rehandshake: not yet implemented"
 
 let rekey s c = FStar.Error.unexpected "rekey: not yet implemented"
 
+//19-09-13 TODO 
 let send_ticket hs app_data =
-  if is_post_handshake hs then
-    let _ = server_Ticket13 hs app_data in true
-  else false
+//if is_post_handshake hs then
+//  let _ = server_Ticket13 hs app_data in true
+//else 
+    false
 
 let request s c = FStar.Error.unexpected "request: not yet implemented"
 
@@ -79,34 +96,190 @@ let invalidateSession hs = ()
 
 (* ------------------ Outgoing -----------------------*)
 
-let next_fragment_bounded (hs:hs) i (max:nat) =
-    trace "next_fragment";
-    let outgoing = HSL.write_at_most hs.log i max in
-    match outgoing, !hs.state with
-    // when the output buffer is empty, we send extra messages in two cases
-    // we prepare the initial ClientHello; or
-    // after sending ServerHello in plaintext, we continue with encrypted traffic
-    // otherwise, we just returns buffered messages and signals
-    | HSL.Outgoing None None false, C_init ->
-      (match client_ClientHello hs with
-      | Error z -> Error z
-      | Correct () -> Correct(HSL.write_at_most hs.log i max))
-    | HSL.Outgoing None None false, S13_sent_ServerHello ->
-      (match server_ServerFinished_13 hs with
-      | Error z -> Error z
-      | Correct () -> Correct(HSL.write_at_most hs.log i max))
-    | HSL.Outgoing None None false, C13_sent_EOED d ocr cfk ->
-      client13_Finished2 hs d ocr cfk;
-      Correct(HSL.write_at_most hs.log i max)
-    | _ -> Correct outgoing // nothing to do
+// We send extra messages in three cases: we prepare the initial
+// ClientHello; or the output buffer is empty, after sending
+// ServerHello in plaintext, we continue with encrypted traffic.
+// Otherwise, we just returns buffered messages and signals.
 
-let next_fragment (hs:hs) i =
+let rec next_fragment_bounded hs i max =
+  trace "next_fragment";
+  match hs with 
+  | Client region config r -> (
+    let st0 = !r in 
+    if C_init? st0 then (
+      match Client.client_ClientHello hs with
+      | Error z -> Error z
+      | Correct () -> next_fragment_bounded hs i max )
+    else 
+      let ms0 = Machine.client_ms st0 in 
+      let sending, result = Send.write_at_most ms0.sending i max in
+      let ms1 = { ms0 with sending = sending } in 
+      let st1 = set_client_ms st0 ms1 in 
+      // any simpler way to update substate? 
+      r := st1; 
+      match result, st1 with
+      | Send.Outgoing None None false, 
+        C13_complete offer sh ee server_id fin1 fin2 (Some _) ms ks -> (
+        match Client.client13_Finished2 hs with
+        | Error z -> Error z 
+        | Correct _ -> next_fragment_bounded hs i max )
+
+      | _ -> Correct result // nothing to do
+    )
+  | Server region config r -> ( 
+    let st0 = !r in 
+    let ms0 = Machine.server_ms st0 in 
+    let sending, result = Send.write_at_most ms0.sending i max in
+    let ms1 = { ms0 with sending = sending } in 
+    let st1 = set_server_ms st0 ms1 in 
+    r := st1; 
+    match result, st1 with
+    | Send.Outgoing None None false, 
+      S13_sent_ServerHello _ _ _ -> (
+      match Server.server_ServerFinished_13 hs with
+      | Error z -> Error z 
+      | Correct _ -> next_fragment_bounded hs i max )
+    | _ -> Correct result // nothing to do
+    )
+
+let next_fragment hs i =
   next_fragment_bounded hs i max_TLSPlaintext_fragment_length
 
-let to_be_written (hs:hs) =
-  HSL.to_be_written hs.log
+let to_be_written hs =
+  let sto = 
+    match hs with
+    | Machine.Client region config r -> 
+      let st = !r in (client_ms st).sending
+    | Server region config r -> 
+      let st = !r in (server_ms st).sending in 
+  Send.to_be_written sto
 
 (* ----------------------- Incoming ----------------------- *)
+
+let buffer_received_fragment ms #i rg f = ms
+
+// Some parsing functions translating between low-level representations
+// obtained after receiving, and high-level values passed as arguments
+// to the processing functions
+// TODO: Implement this. This is likely a well-chosen call to Parsers.ServerHello.something
+assume
+val parse_wait_serverHello
+  (#st:Receive.state)
+  (res:PF.c_wait_ServerHello (Receive.cslice_of st) & UInt32.t) :
+  ST Parsers.ServerHello.serverHello
+    (requires fun h -> PF.valid_c_wait_ServerHello st.Receive.rcv_from (snd res) (fst res) h)
+    // Maybe a bit too strong?
+    (ensures fun h0 _ h1 -> h0 == h1)
+
+#set-options "--max_fuel 0 --max_ifuel 1 --z3rlimit 20"
+// #set-options "--admit_smt_queries true"
+let rec recv_fragment hs #i rg f =
+  let open HandshakeMessages in
+  let recv_again r =
+    match r with
+    // only case where the next incoming flight may already have been buffered.
+    | Receive.InAck false false -> recv_fragment hs #i (0,0) empty_bytes
+    | r -> r  in
+  // trace "recv_fragment";
+  let h0 = HST.get() in
+  match hs with 
+  | Client region config r -> (
+    match !r  with
+    | C_init _ ->
+      Receive.InError (
+        fatalAlert Unexpected_message,
+        "Client hasn't sent hello yet (to be statically excluded)")
+
+    | C_wait_ServerHello offer0 ms0 ks0 -> (
+      // AF: How do we ensure this statically? Should this be handled
+      // by buffer_received_fragment, returning an Error if the
+      // property does not hold? CF: yes; or realloc the buffer if
+      // this is problematic.
+      let rcv0 = ms0.receiving in 
+      assume Receive.(UInt32.v rcv0.rcv_to + Bytes.length f <= UInt32.v rcv0.rcv_b.LP.len);
+      let rcv1 = buffer_received_fragment rcv0 #i rg f in
+      match Receive.receive_c_wait_ServerHello rcv1 with
+      | Error z -> Receive.InError z
+      | Correct (x, rcv2) ->
+        let v = C_wait_ServerHello offer0 ({ms0 with receiving = rcv2}) ks0 in
+        let h1 = HST.get() in
+        r := v;
+        let h2 = HST.get() in
+        match x with
+        | None -> Receive.InAck false false // nothing happened
+        | Some sh_msg -> (
+          let sh = parse_wait_serverHello sh_msg in
+          let h3 = HST.get() in
+          if HSM.is_hrr sh then
+            // TODO adjust digest, here or in the transition call
+            Client.client_HelloRetryRequest hs sh
+          else
+            // TODO extend digest[..sh]
+            // transitioning to C12_wait_ServerHelloDone or C13_wait_Finished1;
+            let r = Client.client_ServerHello hs sh in
+            // TODO check that ms1.receiving is set for processing the next flight
+            recv_again r )))
+(*
+  | C12_wait_ServerHelloDone ch sh ms0 ks -> (
+    let rcv1 = buffer_received_fragment ms0.receiving f in
+    match TLS.Handshake.Receive.receive_c12_wait_ServerHelloDone rcv1 with
+    | Error z -> InError z
+    | Correct (x, rcv2) ->
+      hs.cstate := C12_wait_ServerHelloDone ch sh ({ms0 with receiving = rcv2}) ks;
+      match x with
+      | None -> InAck false false // nothing happened
+      | Some x ->
+      // TODO extend digest[..ServerHelloDone]
+      // let c, ske, ocr = admit() in
+      // client_ServerHelloDone hs c ske None
+        admit()
+      )
+
+  | C13_wait_Finished1 offer sh ms0 ks -> (
+    let rcv1 = buffer_received_fragment ms0.receiving f in
+    match TLS.Handshake.Receive.receive_c13_wait_Finished1 rcv1
+    with
+    | Error z -> InError z
+    | Correct (x, rcv2) ->
+      hs.cstate := C13_wait_Finished1 offer sh ({ms0 with receiving = rcv2}) ks;
+      match x with
+      | None -> InAck false false // nothing happened
+      | Some x ->
+        // covering 3 cases (see old code for details)
+        // we need to extract these high-level values from the flight:
+        let ee, ocr, oc, ocv, fin1, otag0, tag1, tag_fin1 = admit() in
+        client_ServerFinished13 hs offer sh ee ocr oc ocv fin1 otag0 tag1 tag_fin1
+      )
+
+  | C13_Complete _ _ _ _ _ _ _ ms0 _ ->
+    let ms1 = buffer_received_fragment ms0 #i rg f in
+    // TODO two sub-states: waiting for fin2 or for the post-handshake ticket.
+    match HSL.Receive.receive_c_wait_ServerHello 12_wait_ServerHelloDone st b f_begin f_end with
+    | Error z -> InError z
+    | Correct None -> InAck false false // nothing happened
+    | Correct (Some x) ->
+
+  , [Msg13 (M13_new_session_ticket st13)], [_] ->
+      client_NewSessionTicket_13 hs st13
+
+  // 1.2 full: wrap these two into a single received flight with optional [cr]
+    | C_wait_Finished2 digestClientFinished, [Msg12 (M12_finished f)], [digestServerFinished] ->
+      client_ServerFinished hs f digestClientFinished
+
+    | C_wait_NST resume, [Msg12 (M12_new_session_ticket st)], [digestNewSessionTicket] ->
+      client_NewSessionTicket_12 hs resume digestNewSessionTicket st
+
+    // 1.2 resumption
+    | C_wait_R_Finished1 digestNewSessionTicket, [Msg12 (M12_finished f)], [digestServerFinished] ->
+      client_R_ServerFinished hs f digestNewSessionTicket digestServerFinished
+*)
+
+  | _ ->
+    Receive.InError (fatalAlert Unexpected_message, "TBC")
+
+
+
+(* The old, but more complete version, to be merged: 
 
 let rec recv_fragment (hs:hs) #i rg f =
   let open HandshakeLog in
@@ -207,11 +380,13 @@ let rec recv_fragment (hs:hs) #i rg f =
     | _,  _, _ ->
 //      trace "DISCARD FLIGHT"; InAck false false
       InError(fatalAlert Unexpected_message, "unexpected flight")
+*)
 
 // TODO check CCS once committed to TLS 1.3 yields an alert
-let recv_ccs (hs:hs) =
-  let open HandshakeLog in
-  let open HandshakeMessages in
+let recv_ccs hs =
+  admit()
+  //19-09-13 TBC 
+(*  
   trace "recv_ccs";
   // Draft 22 CCS during HRR
   // Because of stateless HRR, this may also happen as the very first message before CH (!!!)
@@ -248,6 +423,7 @@ let recv_ccs (hs:hs) =
       | _, _, _ ->
         trace "WARNING: bad CCS";
         InError(fatalAlert Unexpected_message, "CCS received at wrong time")
+*)
 
 
 let authorize s ch = FStar.Error.unexpected "authorize: not yet implemented"
